wip Modular semantics

src/Prototype/Reduction.v
@@ -1,20 +1,63 @@
 Require Import List String Peano_dec.
-Require Import FnMap Language.
+Require Import FnMap Language Transaction.
 
 Set Implicit Arguments.
 
 Section Reduction.
-  Context {MsgT IStateT SStateT: Type}.
+  Context {MsgT StateT: Type}.
   Context {MvalT: MsgT -> RqRs -> Type}.
   Hypothesis (msgT_dec : forall m1 m2 : MsgT, {m1 = m2} + {m1 <> m2}).
 
+  Local Notation Msg := (Msg MvalT).
   Local Notation MsgId := (MsgId MsgT).
   Local Notation Label := (Label MvalT).
 
-  Definition Reduced (from to: list Label) (lbl1 lbl2: Label) :=
-    exists hst1 hst2,
-      from = hst1 ++ lbl1 :: lbl2 :: hst2 /\
-      to = hst1 ++ lbl2 :: lbl1 :: hst2.
+  Definition History4 (hst: list Msg) (msg1 msg2 msg3 msg4: Msg)
+             (shst1 shst2 shst3 shst4 shst5: list Msg) :=
+    hst = shst5 ++ msg4 :: shst4 ++ msg3 :: shst3 ++ msg2 :: shst2 ++ msg1 :: shst1.
 
+  Definition Interleaving21 (hst: list Msg) (rq1 rs1 rq2 rs2: Msg)
+             (shst1 shst2 shst3 shst4 shst5: list Msg) :=
+    isTrsPair msgT_dec (msg_id rq1) (msg_id rs1) = true /\
+    isTrsPair msgT_dec (msg_id rq2) (msg_id rs2) = true /\
+    History4 hst rq1 rq2 rs1 rs2 shst1 shst2 shst3 shst4 shst5.
+  
+  Definition Interleaving22 (hst: list Msg) (rq1 rs1 rq2 rs2: Msg)
+             (shst1 shst2 shst3 shst4 shst5: list Msg) :=
+    isTrsPair msgT_dec (msg_id rq1) (msg_id rs1) = true /\
+    isTrsPair msgT_dec (msg_id rq2) (msg_id rs2) = true /\
+    History4 hst rq1 rq2 rs2 rs1 shst1 shst2 shst3 shst4 shst5.
+
+  Definition Interleaving2 (hst: list Msg) (rq1 rs1 rq2 rs2: Msg)
+             (shst1 shst2 shst3 shst4 shst5: list Msg) :=
+    Interleaving21 hst rq1 rs1 rq2 rs2 shst1 shst2 shst3 shst4 shst5 \/
+    Interleaving22 hst rq1 rs1 rq2 rs2 shst1 shst2 shst3 shst4 shst5.
+    
+  Definition Sequential2 (hst: list Msg) (rq1 rs1 rq2 rs2: Msg)
+             (shst1 shst2 shst3 shst4 shst5: list Msg) :=
+    isTrsPair msgT_dec (msg_id rq1) (msg_id rs1) = true /\
+    isTrsPair msgT_dec (msg_id rq2) (msg_id rs2) = true /\
+    History4 hst rq1 rs1 rq2 rs2 shst1 shst2 shst3 shst4 shst5.
+
+  Definition Reducible2 (sys: System MvalT StateT) :=
+    forall hst,
+      History sys hst ->
+      forall rq1 rs1 rq2 rs2 shst1 shst2 shst3 shst4 shst5,
+        Interleaving2 hst rq1 rs1 rq2 rs2 shst1 shst2 shst3 shst4 shst5 ->
+        exists hst',
+          History sys hst' /\
+          Sequential2 hst' rq1 rs1 rq2 rs2 shst1 shst2 shst3 shst4 shst5.
+
+  Section Facts.
+
+    Lemma singleton_reducible_linear:
+      forall obj,
+        Reducible2 (obj :: nil) ->
+        Linear msgT_dec (obj :: nil).
+    Proof.
+    Admitted.
+
+  End Facts.
+  
 End Reduction.
-        
+
